add wrapper_correct

wrapper.v
@@ -1,7 +1,6 @@
 From mathcomp Require Import all_ssreflect.
 From Michocoq Require Import semantics util macros.
 Import syntax comparable error.
-Require Import ZArith.
 
 Set Implicit Arguments.
 Unset Strict Implicit.
@@ -64,7 +63,7 @@ Definition exec_correct_success
 (A : instruction_seq None false (pair bytes bytes ::: [::])
                  (pair (list operation) bytes ::: [::]))
 fuel returned_operations new_storage :
-  4 <= fuel ->
+  3 <= fuel ->
   eval_seq (no_self env) A fuel (arg, wstore, tt) = Return (returned_operations, new_storage, tt) ->
   eval_seq env (exec A) fuel.+1 (arg, wstore, avt_id, tt) =
   Return (returned_operations,
@@ -73,7 +72,7 @@ fuel returned_operations new_storage :
            (new_storage, avt_id)), tt).
 Proof.
   move=> Hfuel.
-  have<-: 3 + (fuel - 3) = fuel by rewrite addnC subnK // (ltn_trans _ Hfuel).
+  have<-: 3 + (fuel - 3) = fuel by rewrite addnC subnK.
   by rewrite /eval_seq /= => ->.
 Qed.
 
@@ -85,12 +84,12 @@ Definition exec_correct_fail
 (A : instruction_seq None false (pair bytes bytes ::: [::])
                  (pair (list operation) bytes ::: [::]))
 fuel e :
-  4 <= fuel ->
+  3 <= fuel ->
   eval_seq (no_self env) A fuel (arg, wstore, tt) = Failed _ e ->
   eval_seq env (exec A) fuel.+1 (arg, wstore, avt_id, tt) = Failed _ e.
 Proof.
   move=> Hfuel.
-  have<-: 3 + (fuel - 3) = fuel by rewrite addnC subnK // (ltn_trans _ Hfuel).
+  have<-: 3 + (fuel - 3) = fuel by rewrite addnC subnK.
   by rewrite /eval_seq /= => ->.
 Qed.
 
@@ -102,7 +101,7 @@ Lemma wrapper_correct_success
 (A : instruction_seq None false (pair bytes bytes ::: [::])
                  (pair (list operation) bytes ::: [::]))
 (fuel : Datatypes.nat) returned_operations new_storage :
-  4 <= fuel ->
+  3 <= fuel ->
   eval_seq (no_self env) A fuel (arg, wstore, tt) = Return (returned_operations, new_storage, tt) ->
   eval_seq env wrapper fuel.+1 (arg, ((existT _ false A : data (lambda (pair bytes bytes)
                                          (pair (list operation) bytes))), (wstore, avt_id)), tt)
@@ -111,8 +110,8 @@ Lemma wrapper_correct_success
                                             (pair (list operation) bytes))),
            (new_storage, avt_id)), tt).
   rewrite !return_precond !eval_seq_precond_correct => Hfuel.
-  have<-: 4 + (fuel - 4) = fuel by rewrite addnC subnK.
-  move: (eval_seq_precond_eqv _ (no_self env) false _ _ A (4 + (fuel - 4)) (arg, wstore, tt)
+  have<-: 3 + (fuel - 3) = fuel by rewrite addnC subnK.
+  move: (eval_seq_precond_eqv _ (no_self env) false _ _ A (3 + (fuel - 3)) (arg, wstore, tt)
   (fun '(y, tt) =>
      let (x, _) := y in
      let (_, y1) := y in
@@ -125,7 +124,26 @@ Lemma wrapper_correct_success
   split; by case => -> ->.
 Qed.
 
-Lemma wrapper_correct'
+Lemma wrapper_correct_fail
+(arg : data bytes)
+(wstore : data bytes)
+(avt_id : data (option (pair address (pair syntax_type.string syntax_type.string))))
+(env : @proto_env (Some (parameter_ty, None)))
+(A : instruction_seq None false (pair bytes bytes ::: [::])
+                 (pair (list operation) bytes ::: [::]))
+(fuel : Datatypes.nat) e :
+  3 <= fuel ->
+  eval_seq (no_self env) A fuel (arg, wstore, tt) = Failed _ e ->
+  eval_seq env wrapper fuel.+1 (arg, ((existT _ false A : data (lambda (pair bytes bytes)
+                                         (pair (list operation) bytes))), (wstore, avt_id)), tt)
+= Failed _ e.
+Proof.
+  move=> Hfuel.
+  have<-: 3 + (fuel - 3) = fuel by rewrite addnC subnK.
+  by rewrite /eval_seq /= => ->.
+Qed.
+
+Lemma wrapper_correct
 (arg : data bytes)
 (wstore : data bytes)
 (avt_id : data (option (pair address (pair syntax_type.string syntax_type.string))))
@@ -133,42 +151,14 @@ Lemma wrapper_correct'
 (A : instruction_seq None false (pair bytes bytes ::: [::])
                  (pair (list operation) bytes ::: [::]))
 (fuel : Datatypes.nat) :
-  fuel > 10 ->
-  eval_seq (no_self env) A (7 + (fuel - 7)) (arg, wstore, tt)
-= eval_seq (no_self env) A (fuel - 7) (arg, wstore, tt) ->
-  eval_seq env wrapper fuel (arg, ((existT _ false A : data (lambda (pair bytes bytes)
-                                         (pair (list operation) bytes))), (wstore, avt_id)), tt)
-= eval_seq env (exec A) fuel (arg, wstore, avt_id, tt).
+  3 <= fuel ->
+  eval_seq env wrapper fuel.+1 (arg, ((existT _ false A : data (lambda (pair bytes bytes)
+                                   (pair (list operation) bytes))), (wstore, avt_id)), tt)
+= eval_seq env (exec A) fuel.+1 (arg, wstore, avt_id, tt).
 Proof.
-  move=> Hf sA /=.
-  have?: 6 < fuel by apply/(leq_trans _ Hf).
-  have<-: (fuel - 7) + 7 = fuel by rewrite subnK.
-  suff->: 6 + (fuel - 7 + 7) = 4 + ((fuel - 7 + 7) + 2).
-  rewrite /eval_seq /=.
-set X := RHS.
-
-  rewrite /=.
-  rewrite !bind_id.
-  vm_compute.
-
-  simpl.
-  rewrite /wrapper /=.
-  rewrite /=.
-  rewrite addnC.
-  set A1 := (eval _ A _ _).
-  rewrite /= !bind_id; set A2 := (eval _ A _ _).
-  have->: A1 = A2 by subst A1 A2; rewrite sA.
-  have<-: 4 + ((fuel - 7) - 4) = fuel - 7
-   by rewrite addnC subnK // /leq subnBA // subn_eq0 (leq_trans _ Hf).
-  by case: A2 => []//= [][] /=.
-
-
-  Check eval_seq env A.
-LAMBDA _ _ A;; SWAP;;
-EXEC;; UNPAIR;; DIP1 (PUSH _ (Bytes_constant (pack_lambda A)));;
-DIP1 PAIR;; PAIR.
-
-
-Check (instruction None false (lambda (pair bytes bytes) (pair (list operation) bytes))).
-
+  move=> Hfuel.
+  case HA: (eval_seq (no_self env) A fuel (arg, wstore, tt)) => [e|[][]a b []].
+   by rewrite (@wrapper_correct_fail _ _ _ _ _ _ e) // (@exec_correct_fail _ _ _ _ _ _ e) //.
+   by rewrite (@wrapper_correct_success _ _ _ _ _ _ a b) // (@exec_correct_success _ _ _ _ _ _ a b).
+Qed.
 End wrapper.
